ulib/FStar.SizeT.fsti
@@ -92,6 +92,10 @@ val uint64_to_sizet (x:U64.t) : Pure t
   (requires fits_u64)
   (ensures fun y -> v y == U64.v x)
 
+val sizet_to_uint32 (x:t) : Pure U32.t
+  (requires True)
+  (ensures fun y -> U32.v y == v x % pow2 32)
+
 val fits_lte (x y: nat) : Lemma
   (requires (x <= y /\ fits y))
   (ensures (fits x))
